src/Primitive/Boolean/VstEnc.v
@@ -3,10 +3,14 @@ Require Import Core.Core Core.StructNormalizer VstLib VstCallback
 Require Import VST.floyd.proofauto Psatz.
 Require Import Clight.asn_application Clight.BOOLEAN.
 
+Require Import Core.Notations. 
+
 Definition Vprog : varspecs. mk_varspecs prog. Defined.
 Instance CompSpecs : compspecs. make_compspecs prog. Defined.
+
 Instance Change1 : change_composite_env CompSpecs DWT.Vst.CompSpecs.
 Proof. make_cs_preserve CompSpecs DWT.Vst.CompSpecs. Defined.
+
 Instance Change2 : change_composite_env DWT.Vst.CompSpecs CompSpecs.
 Proof. make_cs_preserve DWT.Vst.CompSpecs CompSpecs. Defined.
 
@@ -16,56 +20,51 @@ Section Boolean_der_encode_primitive.
 
 Definition cb := _overrun_encoder_cb.
 
+Definition bool_of_int (i : int) := 
+  if (i == 0)%int then false else true.
+
 Definition bool_der_encode_spec : ident * funspec :=
   DECLARE _BOOLEAN_encode_der
-    WITH sptr_p : val, sptr_val : Z, gv : globals,
-         (* pointer to the DEF table for the type decoded *)
+    WITH gv : globals,
+         (* parameters : *)
+         res: val,  sptr_p : val, sptr_val : int, 
          td_p : val, td : TYPE_descriptor,
          tag_mode : Z, tag : Z,
-         (* local defs *)
-         b : bool, res : val, b_val : val,
          (* callback pointer *)
-         (*cb_p : val, *)
-         (* callback argument pointer *)
-         app_p : val, app_key_val : val
-    PRE[(* added by clightgen - since returning structs is not supported *) 
-        tptr enc_rval_s, tptr type_descriptor_s, tptr tvoid, tint, 
-        tuint, tptr cb_type, tptr tvoid]
-      PROP((* If I understood this correctly there is an implicit contract
-              on this function, that is, type_descriptor equals bool type 
-              if it was passed here, since there isn't any check on tags for it
-              to be bool. Alternatively there may not be any implicit contract
-              in which case it can lead to malformed output which needs to be
-              checked somewhere. Maybe decoder checks for it... *)
-           decoder_type td = BOOLEAN_t)
-      PARAMS(res; td_p; sptr_p; Vint (Int.repr tag_mode);
-             Vint (Int.repr tag); (gv cb); app_p)
-      GLOBALS(gv)
-      SEP((* td points to td with readable permission *) 
-          data_at_ Tsh enc_rval_s res;
-          data_at_ Tsh type_descriptor_s td_p; 
-          data_at Tsh tint (Vint (int_of_bool b)) sptr_p;
-          data_at_ Tsh tvoid app_p;
-          valid_pointer (gv cb); func_ptr callback (gv cb))
+         (*cb_p : val, *) 
+         (* callback argument pointer *)                    
+         app_key_p : val, app_key_val : val
+    PRE [tptr enc_rval_s, tptr type_descriptor_s, tptr tvoid, tint, 
+         tuint, tptr cb_type, tptr tvoid]
+      PROP (decoder_type td = BOOLEAN_t) (* an implicit contract *)
+      PARAMS (res; td_p; sptr_p; Vint (Int.repr tag_mode);
+             Vint (Int.repr tag); gv cb; app_key_p)
+      GLOBALS (gv)
+      SEP (data_at_ Tsh enc_rval_s res;
+           data_at_ Tsh type_descriptor_s td_p; 
+           data_at Tsh tint (Vint sptr_val) sptr_p;
+           data_at_ Tsh tvoid app_key_p;
+           valid_pointer (gv cb);
+           func_ptr callback (gv cb))
     POST [tvoid]
-      PROP()
-      LOCAL()
-      SEP((* Unchanged by the execution : *)
-          data_at Tsh enc_rval_s 
-                  (match evalErrW (bool_encoder td b) [] with
-                   | Some v => construct_enc_rval (encoded v) (Vint (Int.repr 0))
-                   | None => construct_enc_rval (-1) sptr_p
-                   end) res;
-          data_at_ Tsh type_descriptor_s td_p ; 
-          data_at Tsh tint (Vint (int_of_bool b)) sptr_p ;
-          data_at_ Tsh tvoid app_p ; valid_pointer (gv cb); 
-          func_ptr callback (gv cb); func_ptr' callback (gv cb)).
+      PROP ()
+      LOCAL ()
+      SEP (let res_val := 
+               match evalErrW (bool_encoder td (bool_of_int sptr_val)) [] with
+               | Some v => construct_enc_rval (encoded v) Vzero
+               | None => construct_enc_rval (-1) sptr_p
+               end in
+           data_at Tsh enc_rval_s res_val res;
+           data_at_ Tsh type_descriptor_s td_p ; 
+           data_at Tsh tint (Vint sptr_val) sptr_p ;
+           data_at_ Tsh tvoid app_key_p ; valid_pointer (gv cb); 
+           func_ptr callback (gv cb); func_ptr' callback (gv cb)).
 
 Definition Gprog := ltac:(with_library prog [der_write_tags_spec; callback_spec;
                                                bool_der_encode_spec]).
 
 Definition if_post1 (gv : globals) cb sptr_p res bool_p erval_p td_p tag_mode 
-           tag app_p td b cb_spec := 
+           tag app_key_p td sptr_val cb_spec := 
   PROP(is_pointer_or_null (gv cb))
   LOCAL(gvars gv;
         temp _t'6 (Vint (Int.repr 2)); 
@@ -75,14 +74,14 @@ Definition if_post1 (gv : globals) cb sptr_p res bool_p erval_p td_p tag_mode
         temp __res res; temp _td td_p; temp _sptr sptr_p; 
         temp _tag_mode (Vint (Int.repr tag_mode)); 
         temp _tag (Vint (Int.repr tag)); 
-        temp _cb (gv cb); temp _app_key app_p) 
+        temp _cb (gv cb); temp _app_key app_key_p) 
   SEP(data_at_ Tsh type_descriptor_s td_p; 
-      data_at_ Tsh enc_rval_s res; data_at_ Tsh tvoid app_p; 
+      data_at_ Tsh enc_rval_s res; data_at_ Tsh tvoid app_key_p; 
       func_ptr cb_spec (gv cb); func_ptr' cb_spec (gv cb); 
       (match (gv cb) with
        | Vint _ => data_at_ Tsh tuchar bool_p
        | _ => data_at Tsh tuchar 
-                     (Vubyte (match execErrW (bool_encoder td b) [] with 
+                     (Vubyte (match execErrW (bool_encoder td (bool_of_int sptr_val)) [] with 
                               | Some v => last v (Byte.repr (-1)) 
                               | None => (Byte.repr (-1)) 
                               end)) bool_p end);
@@ -93,10 +92,10 @@ Definition if_post1 (gv : globals) cb sptr_p res bool_p erval_p td_p tag_mode
                erval_p;
       field_at Tsh (Tstruct _asn_enc_rval_s noattr) (DOT _structure_ptr) 
                (default_val (tptr tvoid)) erval_p; 
-      data_at Tsh tint (Vint (int_of_bool b)) sptr_p; 
+      data_at Tsh tint (Vint sptr_val) sptr_p; 
       valid_pointer (gv cb)).
 
-Definition if_post2 (gv : globals) (b : bool) app_p (v_bool_value : val) cb_spec 
+Definition if_post2 (gv : globals) (sptr_val : int) app_key_p (v_bool_value : val) cb_spec 
            cb v_bool_value v_erval td_p res sptr_p tag_mode tag := 
   PROP()
   LOCAL(gvars gv; temp _t'6 (Vint (Int.repr 2));
@@ -106,10 +105,10 @@ Definition if_post2 (gv : globals) (b : bool) app_p (v_bool_value : val) cb_spec
         temp __res res; temp _td td_p; temp _sptr sptr_p;
         temp _tag_mode (Vint (Int.repr tag_mode)); 
         temp _tag (Vint (Int.repr tag)); 
-        temp _cb (gv cb); temp _app_key app_p;
-        temp _t'2 (Vint (Int.repr (if b then 255 else 0))))
+        temp _cb (gv cb); temp _app_key app_key_p;
+        temp _t'2 (Vint (Int.repr (if (bool_of_int sptr_val) then 255 else 0))))
   SEP(data_at_ Tsh type_descriptor_s td_p;
-      data_at_ Tsh tvoid app_p; func_ptr cb_spec (gv cb);
+      data_at_ Tsh tvoid app_key_p; func_ptr cb_spec (gv cb);
       data_at_ Tsh tuchar v_bool_value;
       field_at Tsh (Tstruct _asn_enc_rval_s noattr) (DOT _encoded) 
                (Vint (Int.repr 2)) v_erval;
@@ -119,10 +118,10 @@ Definition if_post2 (gv : globals) (b : bool) app_p (v_bool_value : val) cb_spec
       field_at Tsh (Tstruct _asn_enc_rval_s noattr) (DOT _structure_ptr) 
                (default_val (tptr tvoid)) v_erval; 
       data_at_ Tsh enc_rval_s res;
-      data_at Tsh tint (Vint (int_of_bool b)) sptr_p; valid_pointer (gv cb)).
+      data_at Tsh tint (Vint sptr_val) sptr_p; valid_pointer (gv cb)).
 
 Definition loop_inv (gv : globals) sptr_p v_bool_value v_erval res td_p tag_mode 
-           tag cb app_p (cb_spec : funspec) b :=
+           tag cb app_key_p (cb_spec : funspec) sptr_val :=
   PROP()
   LOCAL(gvars gv; temp _t'4 (Vint (Int.repr 2)); 
         temp _t'6 (Vint (Int.repr 2)); temp _t'1 (Vint (Int.repr 2)); 
@@ -131,12 +130,12 @@ Definition loop_inv (gv : globals) sptr_p v_bool_value v_erval res td_p tag_mode
         temp __res res; temp _td td_p; temp _sptr sptr_p;
         temp _tag_mode (Vint (Int.repr tag_mode));
         temp _tag (Vint (Int.repr tag)); temp _cb (gv cb);
-        temp _app_key app_p)
+        temp _app_key app_key_p)
   SEP(data_at_ Tsh type_descriptor_s td_p;
-      data_at_ Tsh enc_rval_s res; data_at_ Tsh tvoid app_p;
+      data_at_ Tsh enc_rval_s res; data_at_ Tsh tvoid app_key_p;
       func_ptr callback (gv cb);
 func_ptr' callback (gv cb);
-      data_at Tsh tuchar (Vubyte (byte_of_bool b)) v_bool_value;
+      data_at Tsh tuchar (Vubyte (byte_of_bool (bool_of_int sptr_val))) v_bool_value;
       field_at Tsh (Tstruct _asn_enc_rval_s noattr) (DOT _encoded) 
                (Vint (Int.add (Int.repr 2) (Int.repr 1))) v_erval;
       field_at Tsh (Tstruct _asn_enc_rval_s noattr) (DOT _failed_type)  
@@ -144,7 +143,7 @@ func_ptr' callback (gv cb);
                v_erval;
       field_at Tsh (Tstruct _asn_enc_rval_s noattr) (DOT _structure_ptr)
                (default_val (tptr tvoid)) v_erval;
-      data_at Tsh tint (Vint (int_of_bool b)) sptr_p;
+      data_at Tsh tint (Vint sptr_val) sptr_p;
       valid_pointer (gv cb)).
 
 Theorem bool_der_encode : semax_body Vprog Gprog 
@@ -154,35 +153,37 @@ Theorem bool_der_encode : semax_body Vprog Gprog
 Proof.
   start_function; rename H into DT.
   forward.
-  forward_call (td_p, td, 1, tag_mode, 0, tag, (gv cb), app_p, app_key_val).
+  forward_call (td_p, td, 1, tag_mode, 0, tag, (gv cb), app_key_p, app_key_val).
   rewrite Exec.eval_dwt_boolean by assumption.
   unfold_data_at_ v_erval; unfold_data_at (data_at _ _ _ v_erval).
   forward.
   forward.
   forward_if; [contradiction|clear H].
   forward_if (if_post1 gv cb sptr_p res v_bool_value v_erval td_p tag_mode tag 
-                       app_p td b callback); unfold if_post1.
+                       app_key_p td sptr_val callback); unfold if_post1.
   * (* if(cb) = true *)
     forward.
     (* bool_value = *st ? 0xff : 0; /* 0xff mandated by DER */ *)
-    forward_if (if_post2 gv b app_p v_bool_value callback cb v_bool_value 
+    forward_if (if_post2 gv sptr_val app_key_p v_bool_value callback cb v_bool_value 
                          v_erval td_p res sptr_p tag_mode tag); unfold if_post2.
     - (* if(b) = true *)
       forward; unfold if_post2; entailer!.
-      destruct b; [auto|contradiction].
+      unfold bool_of_int.
+      destruct (sptr_val == 0)%int eqn : S; 
+        [eapply int_eq_e in S; contradiction | auto ].
     - (* if(b) = false *)
       forward; unfold if_post2; entailer!.
-      destruct b; unfold int_of_bool in H2; [discriminate|auto].
     - forward.
       make_func_ptr cb.
-      forward_call ([byte_of_bool b], v_bool_value, 1, app_p).
+      forward_call ([sptr_val], v_bool_value, 1, app_key_p).
       forward_if; [congruence|].
       ** (* cb() >= 0 *)
         unfold if_post1; forward.
          entailer!.
          destruct (gv cb); intuition.
          rewrite exec_boolean_enc by assumption.
-         destruct b; entailer!.
+         unfold bool_of_int.
+         destruct (sptr_val == 0)%int eqn : S; entailer!.
   * (* post if *)
     forward; unfold if_post1.
     rewrite H; entailer!.
@@ -193,7 +194,7 @@ Proof.
     forward.
     unfold construct_enc_rval, encoded, last.
     forward_loop (loop_inv gv sptr_p v_bool_value v_erval res td_p tag_mode tag
-                                cb app_p callback b); unfold loop_inv.
+                                cb app_key_p callback sptr_val); unfold loop_inv.
     - entailer!.
       destruct (gv cb); intuition.
     - 
